Sketch the agreement axiom for `tptsto` that we need.

theories/lang/cpp/logic/simple_pred.v
@@ -3,19 +3,17 @@
  *
  * SPDX-License-Identifier: LGPL-2.1 WITH BedRock Exception for use over network, see repository root for details.
  *)
-From iris.base_logic.lib Require Export iprop.
+From iris.algebra Require Import excl gmap.
+From iris.algebra.lib Require Import frac_auth.
+From iris.bi Require Import monpred.
 From iris.bi.lib Require Import fractional.
-Require Import iris.bi.monpred.
-Require Import iris.base_logic.lib.fancy_updates.
-Require Import iris.base_logic.lib.own.
-Require Import iris.base_logic.lib.cancelable_invariants.
-Require Import iris.algebra.lib.frac_auth.
-Require Import iris.algebra.excl.
-Require Import iris.algebra.gmap.
-Require Import iris.proofmode.tactics.
-
+From iris.base_logic.lib Require Export iprop.
+From iris.base_logic.lib Require Import fancy_updates own.
+From iris.base_logic.lib Require Import cancelable_invariants.
+From iris.proofmode Require Import tactics.
+From iris_string_ident Require Import ltac2_string_ident.
 From bedrock.lang.cpp Require Import ast semantics.
-Require Import bedrock.lang.cpp.logic.pred.
+From bedrock.lang.cpp.logic Require Import pred.
 
 Set Default Proof Using "Type".
 
@@ -66,6 +64,17 @@ Definition _Z_to_bytes {σ:genv} (n : nat) (v : Z) : list N :=
   | Big => List.rev little
   end.
 
+Local Lemma length__Z_to_bytes_le {σ} n v :
+  length (_Z_to_bytes_le (σ:=σ) n v) = n.
+Proof. by rewrite /_Z_to_bytes_le fmap_length seq_length. Qed.
+
+Local Lemma length__Z_to_bytes {σ} n v :
+  length (_Z_to_bytes (σ:=σ) n v) = n.
+Proof.
+  rewrite /_Z_to_bytes.
+  by case: (byte_order _); rewrite ?rev_length length__Z_to_bytes_le.
+Qed.
+
 (** soundness proof *)
 
 Module SimpleCPP_BASE <: CPP_LOGIC_CLASS.
@@ -81,8 +90,11 @@ Module SimpleCPP_BASE <: CPP_LOGIC_CLASS.
     (* ^ you need the same pointer and consecutive integers to "have" a pointer.
      *)
 
-  Definition Z_to_bytes {σ:genv} n v :=
+  Definition Z_to_bytes {σ:genv} (n : nat) (v : Z) : list runtime_val :=
     Rval <$> _Z_to_bytes (σ:=σ) n v.
+
+  Lemma length_Z_to_bytes {σ} n v : length (Z_to_bytes (σ:=σ) n v) = n.
+  Proof. by rewrite/Z_to_bytes fmap_length length__Z_to_bytes. Qed.
 
   Class cppG' (Σ : gFunctors) : Type :=
     { memG : inG Σ (gmapR addr (fractionalR (leibnizO runtime_val)))
@@ -153,6 +165,8 @@ Module SimpleCPP.
     Qed.
 
     (** pointer validity *)
+    (** Pointers past the end of an object/array can be valid; see
+    https://eel.is/c++draft/expr.add#4 *)
     Definition valid_ptr (p : ptr) : mpred.
     refine ([| p = nullptr |] \\//
             (Exists base l h o,
@@ -196,6 +210,12 @@ Module SimpleCPP.
       Definition cptr (a : N) : list runtime_val :=
         Z_to_bytes POINTER_BYTES (Z.of_N a).
 
+      Lemma length_aptr p : length (aptr p) = POINTER_BYTES.
+      Proof. by rewrite/aptr fmap_length seq_length. Qed.
+      Lemma length_cptr a : length (cptr a) = POINTER_BYTES.
+      Proof. by rewrite /cptr length_Z_to_bytes. Qed.
+
+      (** WRT pointer equality, see https://eel.is/c++draft/expr.eq#3 *)
       Definition encodes (t : type) (v : val) (vs : list runtime_val) : mpred.
       refine
         match erase_qualifiers t with
@@ -215,12 +235,9 @@ Module SimpleCPP.
           end
 
         | Tbool =>
-          match v with
-          | Vint 0 => [| vs = Rval 0%N :: nil |]
-          | Vint 1 => [| vs = Rval 1%N :: nil |]
-          | Vundef => [| length vs = 1 |]
-          | _ => lfalse
-          end
+          if decide (v = Vint 0) then [| vs = [Rval 0%N] |]
+          else if decide (v = Vint 1) then [| vs = [Rval 1%N] |]
+          else lfalse
         | Tnullptr =>
           [| vs = cptr 0 |]
         | Tfloat _ => lfalse
@@ -231,12 +248,7 @@ Module SimpleCPP.
             if decide (p = nullptr) then
               [| vs = cptr 0 |]
             else
-              Exists (l : option addr),
-                own _ghost.(mem_inj_name) {[ p := to_agree l ]} **
-                match l with
-                | None => [| vs = aptr p |]
-                | Some l => [| vs = cptr l |]
-                end
+              [| vs = aptr p |]
           | _ => lfalse
           end
         | Tfunction _ _
@@ -245,12 +257,7 @@ Module SimpleCPP.
           match v with
           | Vptr p =>
             [| p <> nullptr |] **
-            Exists (l : option addr),
-              own _ghost.(mem_inj_name) {[ p := to_agree l ]} **
-              match l with
-              | None => [| vs = aptr p |]
-              | Some l => [| vs = cptr l |]
-              end
+            [| vs = aptr p |]
           | Vundef => [| length vs = POINTER_BYTES |]
           | _ => lfalse
           end
@@ -263,13 +270,12 @@ Module SimpleCPP.
       all: refine _.
       Defined.
 
-
       Global Instance encodes_persistent : forall t v vs, Persistent (encodes t v vs).
       Proof.
         unfold encodes.
         intros; destruct (erase_qualifiers t); intros;
           destruct v; try refine _.
-        - destruct (decide (p = nullptr)); refine _.
+        - case_decide; refine _.
         - destruct z; refine _.
           destruct p; refine _.
       Qed.
@@ -277,11 +283,52 @@ Module SimpleCPP.
       Global Instance encodes_timeless : forall t v a, Timeless (encodes t v a).
       Proof.
         intros. unfold encodes. destruct (erase_qualifiers t); destruct v; refine _.
-        - destruct (decide (p = nullptr)); refine _.
+        - case_decide; refine _.
         - destruct z; refine _.
           destruct p; refine _.
       Qed.
 
+      Local Hint Resolve bi.False_elim : core.
+      Local Hint Resolve length_Z_to_bytes : core.
+      Local Hint Resolve length_aptr : core.
+      Local Hint Resolve length_cptr : core.
+
+      Lemma length_encodes t v vs :
+        encodes t v vs |-- [|
+          length vs = match erase_qualifiers t with
+          | Tbool => 1
+          | Tint sz _ => size_to_bytes sz
+
+          | Tmember_pointer _ _ | Tnullptr | Tpointer _
+          | Tfunction _ _ | Treference _ | Trv_reference _ =>
+            POINTER_BYTES
+
+          | _ => 0	(* dummy *)
+          end
+        |].
+      Proof.
+        rewrite/encodes. destruct (erase_qualifiers _), v; try done; intros;
+        repeat match goal with
+        | |- [| _ = _ |] |-- [| _ |] => f_equiv=>->
+        | |- [| _ ≠ _ |] ** [| _ = _ |] |-- [| _ |] => rewrite bi.sep_elim_r
+        | |- context [@decide _ _] => case_decide
+        end;
+        auto.
+      Qed.
+
+      Local Hint Extern 1 =>
+        match goal with
+        | |- (False ∗ _ ⊢ _)%I => rewrite bi.sep_elim_l; apply bi.False_elim
+        | |- (_ ∗ False ⊢ _)%I => rewrite bi.sep_elim_r; apply bi.False_elim
+        end : core.
+      Lemma encodes_agree t v1 v2 vs :
+        encodes t v1 vs |-- encodes t v2 vs -* [| v1 = v2 |].
+      Proof.
+        apply bi.wand_intro_r.
+        rewrite/encodes. case: (erase_qualifiers t)=>//=.
+        - move=>_. case: v1; auto=>p1. case: v2; auto=>p2.
+          (* PDS: I see no way to proceed when p1 null, p2 nonnull *)
+      Abort.
     End with_genv.
 
     Instance Z_to_bytes_proper :
@@ -291,39 +338,11 @@ Module SimpleCPP.
       by setoid_rewrite Hσ.
     Qed.
 
-    Local Ltac go_encode X Y :=
-      let ll := fresh in
-      let rr := fresh in
-        iDestruct X as (ll) "[OL ZL]";
-        iDestruct Y as (rr) "[OR ZR]";
-        iDestruct (own_valid_2 with "OL OR") as X;
-        rewrite join_singleton_eq singleton_valid_at_norm
-                agree_validI agree_equivI;
-        iDestruct X as %[];
-        destruct ll; iDestruct "ZL" as "%"; subst; iDestruct "ZR" as %[];
-        iFrame; eauto.
-
-    Theorem encodes_consistent : forall σ t v a b,
-        encodes σ t v a ** encodes σ t v b |-- [| length a = length b |].
+    Theorem encodes_consistent σ t v1 v2 vs1 vs2 :
+        encodes σ t v1 vs1 ** encodes σ t v2 vs2 |-- [| length vs1 = length vs2 |].
     Proof.
-      rewrite /encodes; intros.
-      destruct (erase_qualifiers t); simpl.
-      all: try iIntros "[[] _]".
-      all: destruct v; try iIntros "[[] _]".
-      all: try solve [ iIntros "[-> ->]"; eauto ].
-      { destruct (decide (p = nullptr)).
-        - iIntros "[-> ->]"; eauto.
-        - iIntros "[A B]".
-          go_encode "A" "B". }
-      { iIntros "[[% A] [% B]]".
-        go_encode "A" "B". }
-      { iIntros "[[% A] [% B]]".
-        go_encode "A" "B". }
-      { iIntros "[[% A] [% B]]".
-        go_encode "A" "B". }
-      { destruct z; try (iIntros "[-> ->]"; eauto).
-        destruct p; try (iIntros "[-> ->]"; eauto).
-        all: iIntros "[[] _]". }
+      rewrite !length_encodes.
+      iDestruct 1 as "[%Ha %Hb]". iPureIntro. by rewrite Ha Hb.
     Qed.
 
     Instance cptr_proper :
@@ -345,21 +364,10 @@ Module SimpleCPP.
     Proof.
       do 5 red. intros; subst.
       unfold encodes.
-      destruct (erase_qualifiers y0); eauto.
+      destruct (erase_qualifiers y0); auto.
       all: destruct y1; auto.
       all: try (setoid_rewrite H; reflexivity).
-      { destruct (decide (p = nullptr)); try setoid_rewrite H; eauto.
-        apply bi.exist_mono; intro.
-        destruct a; try setoid_rewrite H; eauto. }
-      { apply bi.sep_mono; eauto.
-        apply bi.exist_mono; intro.
-        destruct a; setoid_rewrite H; eauto. }
-      { apply bi.sep_mono; eauto.
-        apply bi.exist_mono; intro.
-        destruct a; setoid_rewrite H; eauto. }
-      { apply bi.sep_mono; eauto.
-        apply bi.exist_mono; intro.
-        destruct a; setoid_rewrite H; eauto. }
+      { destruct (decide (p = nullptr)); try setoid_rewrite H; auto. }
     Qed.
 
     Definition val_ (a : ptr) (v : val) (q : Qp) : mpred.
@@ -368,6 +376,15 @@ Module SimpleCPP.
     apply (@ghost_memG Σ); apply has_cppG.
     refine _.
     Defined.
+
+    Lemma val_agree a v1 v2 q1 q2 :
+      val_ a v1 q1 |-- val_ a v2 q2 -* ⌜v1 = v2⌝.
+    Proof.
+      apply bi.wand_intro_r.
+      rewrite/val_ -own_op own_valid singleton_op.
+      rewrite uPred.discrete_valid singleton_valid.
+      by f_equiv=>/pair_valid [] _ /= /agree_op_invL'.
+    Qed.
 
     Instance: Fractional (val_ a rv).
     Proof.
@@ -391,6 +408,15 @@ Module SimpleCPP.
     apply (@memG Σ); apply has_cppG.
     refine _.
     Defined.
+
+    Lemma byte_agree a rv1 rv2 q1 q2 :
+      byte_ a rv1 q1 |-- byte_ a rv2 q2 -* ⌜rv1 = rv2⌝.
+    Proof.
+      apply bi.wand_intro_r.
+      rewrite/byte_ -own_op own_valid singleton_op.
+      rewrite uPred.discrete_valid singleton_valid.
+      by f_equiv=>/pair_valid [] _ /= /agree_op_invL'.
+    Qed.
 
     Instance: Fractional (byte_ a rv).
     Proof.
@@ -424,14 +450,36 @@ Module SimpleCPP.
     Theorem byte_consistent a b b' q q' :
       byte_ a b q ** byte_ a b' q' |-- byte_ a b (q + q') ** [| b = b' |].
     Proof.
-      iIntros "[Hb Hb']". iDestruct (own_valid_2 with "Hb Hb'") as %Hv.
-      have {Hv}-> : b = b'.
-      - move: Hv. by rewrite singleton_op singleton_valid=>/frac_valid[].
-      - iFrame. auto.
-     Qed.
+      iIntros "[Hb Hb']".
+      iDestruct (byte_agree with "Hb Hb'") as %->. by iFrame.
+    Qed.
 
     Definition bytes (a : addr) (vs : list runtime_val) (q : Qp) : mpred :=
       ([∗list] o ↦ v ∈ vs, (byte_ (a+N.of_nat o)%N v) q)%I.
+
+    Lemma bytes_nil a q : bytes a [] q -|- emp.
+    Proof. done. Qed.
+
+    Lemma bytes_cons a v vs q :
+      bytes a (v :: vs) q -|- byte_ a v q ** bytes (N.succ a) vs q.
+    Proof.
+      rewrite /bytes big_sepL_cons/=. do 2!f_equiv.
+      - lia.
+      - move=>o v'. f_equiv. lia.
+    Qed.
+
+    Lemma bytes_agree a vs1 vs2 q1 q2 :
+      length vs1 = length vs2 →
+      bytes a vs1 q1 ⊢ bytes a vs2 q2 -∗ ⌜vs1 = vs2⌝.
+    Proof.
+      revert a vs2. induction vs1 as [ |v vs1 IH]=>a vs2.
+      { intros ->%symmetry%nil_length_inv. auto. }
+      destruct vs2 as [ |v' vs2]; first done. intros [= Hlen].
+      rewrite !bytes_cons.
+      iIntros "[Hv Hvs1] [Hv' Hvs2] /=".
+      iDestruct (byte_agree with "Hv Hv'") as %->.
+      by iDestruct (IH _ _ Hlen with "Hvs1 Hvs2") as %->.
+    Qed.
 
     Instance: Timeless (bytes a rv q).
     Proof. unfold bytes. intros; refine _. Qed.
@@ -449,22 +497,9 @@ Module SimpleCPP.
     Theorem bytes_consistent : forall q q' b b' a, length b = length b' ->
         bytes a b q ** bytes a b' q' |-- bytes a b (q + q') ** [| b = b' |].
     Proof.
-      unfold bytes.
-      induction b; simpl; intros.
-      - destruct b'. simpl.
-        unfold bytes. simpl. eauto.
-        inversion H.
-      - destruct b'. inversion H.
-        inversion H. simpl.
-        simpl in *.
-        enough (forall n, a0 + N.pos (Pos.of_succ_nat n) = (a0 + 1 + N.of_nat n))%N.
-        2: { intros. lia. }
-        iIntros "[[A B] [C D]]".
-        iDestruct ((IHb b' (a0 + 1)%N H1) with "[B D]") as "[Z ->]".
-        setoid_rewrite H0. iFrame.
-        iDestruct (byte_consistent with "[A C]") as "[ZZ ->]". iFrame.
-        setoid_rewrite H0.
-        assert (r :: b' = r :: b') by reflexivity. iFrame "∗%".
+      intros. iIntros "[Hb Hb']".
+      iDestruct (bytes_agree with "Hb Hb'") as %->; auto.
+      by iFrame "Hb Hb' %".
     Qed.
 
     (* heap points to *)
@@ -493,7 +528,6 @@ Module SimpleCPP.
       intros σ1 σ2 Hσ ??-> ??-> ??-> ??->.
       split'; eapply tptsto_mono; eauto; apply Hσ.
     Qed.
-
 
     Theorem tptsto_fractional :
       forall {σ} ty p v, Fractional (λ q, @tptsto σ ty q p v).
@@ -546,6 +580,23 @@ Module SimpleCPP.
     Proof.
       intros. unfold tptsto. apply _.
     Qed.
+
+    Theorem tptsto_agree : forall σ t q1 q2 p v1 v2,
+        @tptsto σ t q1 p v1 ** @tptsto σ t q2 p v2 |-- [| v1 = v2 |].
+    Proof.
+      iDestruct 1 as "[H1 H2]".
+      iDestruct "H1" as (ma1) "(%Ht1 & Hp1 & Hv1)".
+      iDestruct "H2" as (ma2) "(%Ht2 & Hp2 & Hv2)".
+      iDestruct (own_valid_2 with "Hp1 Hp2") as "%Hv". iClear "Hp1 Hp2".
+      move: Hv. rewrite singleton_op singleton_valid=>/agree_op_invL' ->.
+      case: ma2=>[a| ]; last by iDestruct (val_agree with "Hv1 Hv2") as %->.
+      iDestruct "Hv1" as (vs1) "[He1 Hb1]".
+      iDestruct "Hv2" as (vs2) "[He2 Hb2]".
+      iDestruct (encodes_consistent _ _ _ _ vs1 vs2 with "[He1 He2]") as %?; auto.
+      iDestruct (bytes_agree with "Hb1 Hb2") as %->; auto. iClear "Hb1 Hb2".
+      (* PDS: I see no way to proceed. The preceding lemma
+      [encodes_agree] seems unsound wrt the present ghost state. *)
+    Abort.
 
     Theorem tptsto_has_type : forall σ t q p v,
         @tptsto σ t q p v |-- @tptsto σ t q p v ** [| has_type v t |].
